program-schedule-encoding/functional-induction-proof.v
@@ -1,0 +1,50 @@
+
+
+(* Me proving statements about maps to understand how to use maps in Coq *)
+
+Require Import FunInd.
+Require Import Coq.Lists.List.
+Require Import Coq.FSets.FMapInterface.
+Require Import FMapFacts.
+Require Import FunInd FMapInterface.
+
+
+Require Import
+        Coq.FSets.FMapList
+        Coq.Structures.OrderedTypeEx.
+
+Module Import MNat := FMapList.Make(Nat_as_OT).
+Module Import MNatFacts := WFacts(MNat).
+
+
+
+Module Import OTF_Nat := OrderedTypeFacts Nat_as_OT.
+Module Import KOT_Nat := KeyOrderedType Nat_as_OT.
+(* Consider using https://coq.inria.fr/library/Coq.FSets.FMapFacts.html *)
+(* Consider using https://coq.inria.fr/library/Coq.FSets.FMapFacts.html *)
+(* Consider using https://coq.inria.fr/library/Coq.FSets.FMapFacts.html *)
+
+Definition NatToNat := MNat.t nat.
+Definition NatToNatEmpty : NatToNat := MNat.empty nat.
+
+(* We wish to show that map will have only positive values *)
+Function insertNats (n: nat)  (mm: NatToNat)  {struct n}: NatToNat :=
+  match n with
+  | O => mm
+  | S (next) => insertNats  next (MNat.add n n mm)
+  end.
+
+Theorem insertNatsDoesNotDeleteKeys:
+  forall (n: nat) (k: nat) (mm: NatToNat),
+    MNat.In k mm -> MNat.In k (insertNats n mm).
+  intros n.
+  intros k mm.
+  intros kinmm.
+  functional induction insertNats n mm.
+  exact kinmm.
+  rewrite add_in_iff in IHn0.
+  assert(S next = k \/ MNat.In k mm).
+  auto.
+  apply IHn0.
+  exact H.
+Qed.
