program-schedule-encoding/maps-how-to.v
@@ -1,0 +1,74 @@
+
+(* Me proving statements about maps to understand how to use maps in Coq *)
+
+Require Import FunInd.
+Require Import Coq.Lists.List.
+Require Import Coq.FSets.FMapInterface.
+Require Import FMapFacts.
+Require Import FunInd FMapInterface.
+
+
+Require Import
+  Coq.FSets.FMapList
+  Coq.Structures.OrderedTypeEx.
+
+Module Import MNat := FMapList.Make(Nat_as_OT).
+Module Import MNatFacts := WFacts(MNat).
+
+
+
+Module Import OTF_Nat := OrderedTypeFacts Nat_as_OT.
+Module Import KOT_Nat := KeyOrderedType Nat_as_OT.
+(* Consider using https://coq.inria.fr/library/Coq.FSets.FMapFacts.html *)
+(* Consider using https://coq.inria.fr/library/Coq.FSets.FMapFacts.html *)
+(* Consider using https://coq.inria.fr/library/Coq.FSets.FMapFacts.html *)
+
+Definition NatToNat := MNat.t nat.
+Definition NatToNatEmpty : NatToNat := MNat.empty nat.
+
+(* We wish to show that map will have only positive values *)
+Function insertNats (n: nat)  (mm: NatToNat)  {struct n}: NatToNat :=
+  match n with
+  | O => mm
+  | S (next) => insertNats  next (MNat.add n n mm)
+  end.
+
+Theorem insertNatsDoesNotDelete: forall (n: nat) (k: nat) (mm: NatToNat), MNat.In k mm -> MNat.In k (insertNats n mm).
+  intros n. induction n.
+  intros k mm.
+  intros kinmm.
+  simpl.
+  exact kinmm.
+  intros k mm.
+  intros k_in_mm.
+
+
+
+Example keys_nonnegative: forall (n: nat) (mm: NatToNat), 
+    forall (k: nat),
+      (MNat.In k mm -> k >= 0) -> 
+      (MNat.In k (insertNats n mm)) -> k >= 0.
+Proof.
+  intros n.
+  induction n.
+  intros mm k kinmm.
+  intros in_oldk.
+  simpl in in_oldk.
+  apply kinmm in in_oldk.
+  intuition.
+  intros mm k kinmm.
+  intros in_insertnats_mm.
+  rewrite elements_in_iff in in_insertnats_mm.
+  destruct in_insertnats_mm.
+  rewrite <- elements_mapsto_iff in H.
+  simpl in H.
+
+  assert (k = S n /\ MNat.In k mm).
+  rewrite -> add_mapsto_iff in H.
+
+  (* Now what?? *)
+
+  (* Either k = (Sn) or K \in mm. If k = Sn then k > 0.
+     if k \in mm, then use kinmm. But, how do I split these two cases? *)
+
+  Admitted.
