program-schedule-encoding/maps.v
@@ -1,0 +1,78 @@
+
+(* Me proving statements about maps to understand how to use maps in Coq *)
+
+Require Import FunInd.
+Require Import Coq.Lists.List.
+Require Import Coq.Lists.ListSet.
+Require Import Coq.ZArith.BinInt.
+Require Import Coq.ZArith.BinIntDef.
+Require Import Coq.Numbers.BinNums.
+Require Import Coq.Lists.List.
+Require Import Coq.ZArith.Zbool.
+Require Import Coq.Sorting.Permutation.
+Require Import Coq.Logic.FunctionalExtensionality.
+Require Import Omega.
+Require Import Coq.Bool.Sumbool.
+Require Import Coq.ZArith.Zhints.
+Require Import Coq.Classes.EquivDec.
+Require Import Coq.Structures.Equalities.
+Require Import Coq.FSets.FMapInterface.
+Require Import FMapAVL.
+Require Import Coq.Logic.FinFun.
+
+(* thank you kind stranger for showing me functorial modules syntax *)
+(* http://newartisans.com/2016/10/using-fmap-in-coq/ *)
+
+Require Import
+  Coq.FSets.FMapList
+  Coq.Structures.OrderedTypeEx.
+
+Module Import MNat := FMapList.Make(Nat_as_OT).
+
+
+Require Import
+        Coq.FSets.FMapFacts.
+
+Definition Time := nat.
+Definition IxToTime := MNat.t Time.
+Definition IxToIx := MNat.t Z.
+Definition NatToNat := MNat.t nat.
+
+Definition IxToTimeMempty : IxToTime := MNat.empty Time.
+
+Example correct :(add 1 1 IxToTimeMempty = add 1 1 IxToTimeMempty).
+Proof.
+  reflexivity.
+Qed.
+
+Definition keys (mm: IxToTime) : list nat :=
+  List.map  fst (elements mm).
+
+
+(* Check if you can prove anything about key/value pairs *)
+Definition Map1 := add (10) 1 IxToTimeMempty.
+
+Example keys_nonegative:  forall (k: nat), List.In k (keys Map1) ->  (k <= 20).
+Proof.
+  intros k.
+  intros belong.
+  (* Interesting, simpl seems to be quite good at this type of reasoning *)
+  simpl in belong.
+  destruct belong.
+  omega.
+  tauto.
+Qed.
+
+Definition NatToNatEmpty : NatToNat := MNat.empty nat.
+
+(* We wish to show that map will have only positive values *)
+Function idMapsGo (mm: NatToNat)  (n: nat) {struct n}: NatToNat :=
+  match n with
+  | O => mm
+  | S (next) => idMapsGo (MNat.add n n mm) next
+  end.
+
+Example keys_nonnegative: forall (n: nat), forall (k: nat), List.In k (keys (idMapsGo NatToNatEmpty n)) -> k >= 0.
+Proof.
+  intros n k.
+  functional induction (idMapsGo NatToNatEmpty n).
