program-schedule-encoding/proof.v
@@ -1,0 +1,183 @@
+Require Import Coq.Lists.List.
+Require Import FunInd.
+Require Import Coq.Lists.ListSet.
+Require Import Coq.ZArith.BinInt.
+Require Import Coq.ZArith.BinIntDef.
+Require Import Coq.Numbers.BinNums.
+Require Import Coq.Lists.List.
+Require Import Coq.ZArith.Zbool.
+Require Import Coq.Sorting.Permutation.
+Require Import Coq.Logic.FunctionalExtensionality.
+Require Import Omega.
+Require Import Coq.Bool.Sumbool.
+Require Import Coq.ZArith.Zhints.
+Require Import Coq.Classes.EquivDec.
+Require Import Coq.Structures.Equalities.
+Require Import Coq.FSets.FMapInterface.
+Require Import FMapAVL.
+Require Import FMapFacts.
+Require Import Coq.Logic.FinFun.
+Require Import Nat.
+Require Import VectorDef.
+Require Import MSetWeakList.
+
+(* thank you kind stranger for showing me functorial modules syntax *)
+(* http://newartisans.com/2016/10/using-fmap-in-coq/ *)
+
+Require Import
+  Coq.FSets.FMapList
+  Coq.Structures.OrderedTypeEx.
+
+Module Import M := FMapList.Make(Z_as_OT).
+Module Import MFacts := WFacts(M).
+
+
+
+Require Import
+  Coq.FSets.FMapFacts.
+
+(*Module P := WProperties_fun N_as_OT M.
+*)
+
+
+
+(* An index into memory *)
+Definition MemIx := Z.
+
+(* values in memory *)
+Definition MemValue := Z.
+
+(* factor used in building expressions *)
+(*Inductive Factor : Set := Raw : MemValue -> Factor. *)
+
+(* A statement in our grammar *)
+Inductive Stmt :  Type :=
+  Write : MemIx -> MemValue -> Stmt.
+
+(* Memory is a function from an index to a value *)
+Definition Memory :=  MemIx -> MemValue.
+
+(* initial state of memory *)
+Definition initMemory : Memory := fun ix => Z0.
+
+Theorem initMemoryAlwaysZero : forall (wix: MemIx), (initMemory wix) = Z0.
+Proof.
+  auto.
+Qed.
+
+
+Definition writeToMemory (wix: MemIx) (wval: MemValue) (mold: Memory) : Memory :=
+  fun ix => if (ix =? wix)%Z then wval else mold ix.
+
+Theorem readFromWriteIdentical : forall (wix: MemIx) (wval: MemValue) (mem: Memory),
+    (writeToMemory wix wval mem) wix = wval.
+Proof.
+  intros wix wval mem.
+  unfold writeToMemory.
+  rewrite Z.eqb_refl.
+  reflexivity.
+Qed.
+
+
+(* I do not know who Zneq_to_neq fails. TODO: debug this *)
+Theorem readFromWriteDifferent : forall (wix: MemIx) (rix: MemIx) (wval : MemValue) (mem: Memory),
+    rix <> wix -> (writeToMemory wix wval mem) rix = mem rix.
+Proof.
+  intros wix rix wval mem.
+  intros rix_neq_wix.
+  unfold writeToMemory.
+  assert((rix =? wix)%Z = false).
+  apply Z.eqb_neq in rix_neq_wix.
+  auto.
+  rewrite H.
+  reflexivity.
+Qed.
+
+
+  
+
+(* Model the effect of memory writes on memory. *)
+Definition modelStmtMemorySideEffect (s: Stmt) (mold: Memory) : Memory :=
+  match s with
+  | Write wix wval => (writeToMemory wix wval mold)
+  end.
+
+
+
+(**** Schedule stuff for later, I know nothing on how to prove this stuff ****)
+(* A timepoint for a schedule *)
+
+(* We shouldn't think of this as an actual list, we should think of the list indeces
+as indeces for the schedule to operate on *)
+Definition Stmts (n: nat) := Vector.t Stmt n.
+
+Definition timepoint  (k: nat) (n: nat) := (k < n).
+
+
+Definition ScheduleFn (n: nat) : Type := forall (k1 k2: nat), timepoint k1 n -> timepoint k2 n.
+
+Inductive Schedule (n: nat) (f: ScheduleFn n): Type :=
+ |  mkSchedule: Bijective f -> Schedule n f.
+
+Definition Program (n: nat) (f: ScheduleFn n) := prod (Stmts n) (Schedule n f).
+
+Definition programStmts (n: nat) (f: ScheduleFn n) (p: Program n f) : Stmts n := fst p.
+
+
+(* get ith instruction from a program *)
+Definition programIthInstr  (n: nat) (f: ScheduleFn n) (p: Program n f) (i: timepoint n) : Stmt :=
+   nth (fst p) i.
+
+
+Inductive dependence :=
+| mkDependence: nat -> nat -> dependence.
+
+(* If there is a write to wix at this timepoint t, return [t], else return [] *)
+Definition getWriteAtTimepoint (n: nat) (f: ScheduleFn n) (p: Program n f) (wix_needle: MemIx) (tp: timepoint n) : list (timepoint n) :=
+  match programIthInstr n f p tp with
+  | Write wix _ => if (wix =? wix_needle)%Z
+                   then tp::List.nil
+                   else List.nil
+  end.
+
+
+Theorem n_minus_1_lt_n (n: nat)  : n > 1 -> n - 1 < n.
+  intros.
+  induction n.
+  inversion H.
+  simpl. omega.
+Qed.
+
+(* need to match with witness for why n = 1 or n > 1
+Definition decTimepoint (n: nat) (t: timepoint n) : timepoint n :=
+  match t with
+  | Fin.F1 => Fin.F1
+  | Fin.FS prev => Fin.of_nat_lt (n_minus_1_lt_n n)
+  end.
+*)
+                
+
+Definition decTimepoint (n: nat) (t: timepoint n) : timepoint n := t.
+
+Function getWritesTillTimepointGo (n: nat)
+           (f: ScheduleFn n)
+           (p: Program n f)
+           (wix_needle: MemIx)
+           (tcur: timepoint n) : list (timepoint n) :=
+  match tcur with
+  | Fin.F1 => getWriteAtTimepoint n f p wix_needle tcur
+  | Fin.FS _ =>  let writeAtPrevTimepoints := getWritesTillTimepointGo n f p wix_needle (decTimepoint _ tcur) in writeAtPrevTimepointss
+
+  end.
+
+
+
+Definition makeDependences (n: nat) (f: ScheduleFn n) (p: Program n f) : list dependence :=
+  match programStmts n f p with
+  | Vector.nil _ => List.nil
+  | cons _ s _ rest =>  match s with
+                        | Write wix _ => List.nil
+                        end
+  end.
+
+
