program-schedule-encoding/question.md
@@ -1,0 +1,48 @@
+I'm trying to learn to use the `ListMap` module in Coq. I'm really not sure about proving properties about the keys or values in a `ListMap`, when the `ListMap` is created by a recursive function. I feel like I do not know what tactics to use.
+
+
+    (* Me proving statements about maps to understand how to use maps in Coq *)
+    
+    Require Import FunInd.
+    Require Import Coq.Lists.List.
+    Require Import Coq.FSets.FMapInterface.
+    
+    
+    Require Import
+      Coq.FSets.FMapList
+      Coq.Structures.OrderedTypeEx.
+    
+    Module Import MNat := FMapList.Make(Nat_as_OT).
+    Require Import
+            Coq.FSets.FMapFacts.
+    
+    Definition NatToNat := MNat.t nat.
+    Definition NatToNatEmpty : NatToNat := MNat.empty nat.
+    
+    (* We wish to show that map will have only positive values *)
+    Function insertNats (n: nat)  (mm: NatToNat)  {struct n}: NatToNat :=
+      match n with
+      | O => mm
+      | S (next) => insertNats  next (MNat.add n n mm)
+      end.
+    
+    
+    Definition keys (mm: NatToNat) : list nat :=
+      List.map  fst (elements mm).
+    
+    (* vvvvv How do I prove this? Intuitively it is true *)
+    Example keys_nonnegative: forall (n: nat),
+        forall (k: nat),
+          List.In k (keys (insertNats n NatToNatEmpty)) -> k >= 0.
+    Proof.
+      intros n k in_proof.
+      induction n.
+      simpl in in_proof. tauto.
+      (* ??? NOW WHAT *)
+    Admitted.
+
+Informally, the argument I would use for the below program is that because `n >= 0` because it is a `nat`, the keys inserted into the map by `idMapsGo` will also always be non-negative.
+
+I need to induct on `n` for `keys_nonnegative`. On the `nth` step, we add a key `n`, which will be non-negative (due to being a `nat`). The base case is trivial. 
+
+However, I am unable to convert this intuition into a Coq proof :)
